some minor tweaks

examples/separationLogic/src/smallfoot/Parsetree.sml
@@ -3,6 +3,7 @@ type a_component = string
 datatype a_expression =
     Aexp_ident of string
   | Aexp_num of int
+  | Aexp_hol of string
   | Aexp_uminus of a_expression
   | Aexp_infix of string * a_expression * a_expression
 	  (* string is one of "+", "-", "*", "/", "%" *)
